backend/Mach.v
@@ -548,27 +548,19 @@ Fixpoint make_arguments (rs: regset) (m: mem) sp (al: list (rpair loc)) (lv: lis
   | _, _ => None
  end.
 
-Fixpoint stack_bounds ll :=
-  match ll with
-  | nil => (0, 0)
-  | R _ :: ll' => stack_bounds ll'
-  | S _ ofs ty :: ll' => let '(lo, hi) := stack_bounds ll' in
-      let bofs := Stacklayout.fe_ofs_arg + 4 * ofs in
-      (Z.min lo bofs, Z.max hi (bofs + size_chunk (chunk_of_type ty)))
-  end.
-
 (* When we spawn a thread, it should have a stack frame under it with its arguments. *)
 Inductive entry_point (p: program): mem -> state -> val -> list val -> Prop :=
-  | entry_point_intro: forall b m0 f0 f rs m args lo hi m1 stk,
+  | entry_point_intro: forall b f b0 f0 rs m0 m1 m args,
       let ge := Genv.globalenv p in
-      stack_bounds (regs_of_rpairs (loc_arguments (funsig f))) = (lo, hi) ->
-      Mem.alloc m0 lo hi = (m1, stk) ->
-      Mem.mem_wd m ->
-      Mem.arg_well_formed args m ->
-      globals_not_fresh ge m ->
+      Mem.mem_wd m0 ->
+      globals_not_fresh ge m0 ->
+      Mem.arg_well_formed args m0 ->
       Genv.find_funct_ptr ge b = Some f ->
+      Mem.mem_inj (Mem.flat_inj (Mem.nextblock m0)) m0 m1 ->
+      let stk := Mem.nextblock m0 in
       make_arguments (Regmap.init Vundef) m1 (Vptr stk Ptrofs.zero) (loc_arguments (funsig f)) args = Some (rs, m) ->
-      entry_point p m0 (Callstate (Stackframe f0 (Vptr stk Ptrofs.zero) Vnullptr nil :: nil) b rs m) (Vptr b (Ptrofs.zero)) args.
+      Genv.find_funct_ptr ge b0 = Some (Internal f0) ->
+      entry_point p m0 (Callstate (Stackframe b0 (Vptr stk Ptrofs.zero) Vnullptr nil :: nil) b rs m) (Vptr b (Ptrofs.zero)) args.
 
 Inductive final_state: state -> int -> Prop :=
   | final_state_intro: forall rs m r retcode,
